books/projects/x86isa/proofs/utilities/system-level-mode/paging-defs.lisp
@@ -1,0 +1,459 @@
+;; AUTHOR:
+;; Shilpi Goel <shigoel@cs.utexas.edu>
+
+(in-package "X86ISA")
+(include-book "physical-memory-utils")
+(include-book "gl-lemmas")
+(include-book "clause-processors/find-subterms" :dir :system)
+
+(local (include-book "centaur/bitops/ihs-extensions" :dir :system))
+(local (include-book "centaur/bitops/signed-byte-p" :dir :system))
+
+(local (in-theory (e/d* () (signed-byte-p unsigned-byte-p))))
+
+;; ======================================================================
+
+(defsection reasoning-about-page-tables
+  :parents (proof-utilities)
+
+  :short "Reasoning about paging data structures"
+
+  :long "<p>WORK IN PROGRESS...</p>
+
+<p>This doc topic will be updated in later commits...</p>"
+  )
+
+(defsection paging-defs
+  :parents (reasoning-about-page-tables)
+
+  :long "<p>WORK IN PROGRESS...</p>
+
+<p>This doc topic will be updated in later commits...</p>"
+  )
+
+(local (xdoc::set-default-parents paging-defs))
+
+;; ======================================================================
+
+;; Some misc. lemmas:
+
+(defthm combine-bytes-of-list-combine-bytes
+  (equal (combine-bytes (list (combine-bytes xs)))
+         (combine-bytes xs))
+  :hints (("Goal" :in-theory (e/d* (combine-bytes) (force (force))))))
+
+;; ======================================================================
+
+;; Normalizing memory reads:
+
+(local
+ (defthm dumb-integerp-of-mem
+   (implies (x86p x86)
+            (integerp (xr :mem index x86)))))
+
+(defthm rm08-to-rb
+  (implies (and (x86p x86)
+                (force (canonical-address-p lin-addr)))
+           (equal (rm08 lin-addr r-w-x x86)
+                  (b* (((mv flg bytes x86)
+                        (rb (create-canonical-address-list 1 lin-addr) r-w-x x86))
+                       (result (combine-bytes bytes)))
+                    (mv flg result x86))))
+  :hints (("Goal"
+           :use ((:instance rb-and-rm08-in-programmer-level-mode (addr lin-addr)))
+           :in-theory (e/d* (rm08 rb ifix)
+                            (rb-1 signed-byte-p
+                                  unsigned-byte-p
+                                  force (force))))))
+
+(defthm rm16-to-rb
+  ;; Why don't we need (x86p x86) here?
+  (implies (and (force (canonical-address-p lin-addr))
+                (force (canonical-address-p (+ 1 lin-addr))))
+           (equal (rm16 lin-addr r-w-x x86)
+                  (b* (((mv flg bytes x86)
+                        (rb (create-canonical-address-list 2 lin-addr) r-w-x x86))
+                       (result (combine-bytes bytes)))
+                    (mv flg result x86))))
+  :hints (("Goal"
+           :in-theory (e/d* (rm16 rm08 ifix)
+                            (cons-equal
+                             signed-byte-p
+                             unsigned-byte-p
+                             bitops::logior-equal-0
+                             (:meta acl2::mv-nth-cons-meta)
+                             force (force))))))
+
+(defthm rm32-to-rb
+  (implies (and (force (canonical-address-p lin-addr))
+                (force (canonical-address-p (+ 3 lin-addr)))
+                (x86p x86))
+           (equal (rm32 lin-addr r-w-x x86)
+                  (b* (((mv flg bytes x86)
+                        (rb (create-canonical-address-list 4 lin-addr) r-w-x x86))
+                       (result (combine-bytes bytes)))
+                    (mv flg result x86))))
+  :hints (("Goal"
+           :in-theory (e/d* (rm32 rm08)
+                            (signed-byte-p
+                             unsigned-byte-p
+                             bitops::logior-equal-0
+                             force (force))))))
+
+(defthm rm64-to-rb
+  (implies (and (force (canonical-address-p lin-addr))
+                (force (canonical-address-p (+ 7 lin-addr)))
+                (force (x86p x86)))
+           (equal (rm64 lin-addr r-w-x x86)
+                  (b* (((mv flg bytes x86)
+                        (rb (create-canonical-address-list 8 lin-addr) r-w-x x86))
+                       (result (combine-bytes bytes)))
+                    (mv flg result x86))))
+  :hints (("Goal"
+           :expand ((create-canonical-address-list 8 lin-addr)
+                    (create-canonical-address-list 7 (+ 1 lin-addr))
+                    (create-canonical-address-list 6 (+ 2 lin-addr))
+                    (create-canonical-address-list 5 (+ 3 lin-addr)))
+           :in-theory (e/d* (rm64)
+                            ((:linear bitops::logior-<-0-linear-2)
+                             (:linear ash-monotone-2)
+                             (:rewrite bitops::ash-<-0)
+                             (:rewrite acl2::natp-when-integerp)
+                             cons-equal
+                             signed-byte-p
+                             unsigned-byte-p
+                             bitops::logior-equal-0
+                             (:meta acl2::mv-nth-cons-meta)
+                             force (force))))))
+
+;; ======================================================================
+
+;; Normalizing memory writes:
+
+(defthm xr-mem-write-to-physical-memory-disjoint
+  (implies (not (member-p index p-addrs))
+           (equal (xr :mem index (write-to-physical-memory p-addrs bytes x86))
+                  (xr :mem index x86)))
+  :hints (("Goal" :in-theory (e/d* (member-p) (force (force))))))
+
+(defthm wm08-to-wb
+  (implies (and (force (canonical-address-p lin-addr))
+                (force (unsigned-byte-p 8 byte)))
+           (equal (wm08 lin-addr byte x86)
+                  (wb (create-addr-bytes-alist
+                       (create-canonical-address-list 1 lin-addr)
+                       (list byte))
+                      x86)))
+  :hints (("Goal" :in-theory (e/d* (wm08 wvm08 wb)
+                                   (signed-byte-p
+                                    unsigned-byte-p
+                                    force (force))))))
+
+(defthm wm16-to-wb
+  (implies (and (force (canonical-address-p lin-addr))
+                (force (canonical-address-p (1+ lin-addr))))
+           (equal (wm16 lin-addr word x86)
+                  (wb (create-addr-bytes-alist
+                       (create-canonical-address-list 2 lin-addr)
+                       (byte-ify 2 word))
+                      x86)))
+  :hints (("Goal" :in-theory (e/d* (wm16 wb byte-ify)
+                                   (signed-byte-p
+                                    unsigned-byte-p
+                                    force (force))))))
+
+(defthm wm32-to-wb
+  (implies (and (force (canonical-address-p lin-addr))
+                (force (canonical-address-p (+ 3 lin-addr))))
+           (equal (wm32 lin-addr dword x86)
+                  (wb (create-addr-bytes-alist
+                       (create-canonical-address-list 4 lin-addr)
+                       (byte-ify 4 dword))
+                      x86)))
+  :hints (("Goal" :in-theory (e/d* (wm32 wb byte-ify)
+                                   (signed-byte-p
+                                    unsigned-byte-p
+                                    force (force))))))
+
+(defthm wm64-to-wb
+  (implies (and (force (canonical-address-p lin-addr))
+                (force (canonical-address-p (+ 7 lin-addr))))
+           (equal (wm64 lin-addr qword x86)
+                  (wb (create-addr-bytes-alist
+                       (create-canonical-address-list 8 lin-addr)
+                       (byte-ify 8 qword))
+                      x86)))
+  :hints (("Goal"
+           :expand ((create-canonical-address-list 8 lin-addr)
+                    (create-canonical-address-list 7 (+ 1 lin-addr))
+                    (create-canonical-address-list 6 (+ 2 lin-addr))
+                    (create-canonical-address-list 5 (+ 3 lin-addr)))
+           :in-theory (e/d* (wm64 wb byte-ify)
+                            (signed-byte-p
+                             unsigned-byte-p
+                             force (force))))))
+
+;; ======================================================================
+
+;; Lemmas to aid in symbolic simulation:
+
+(defthmd rm08-in-terms-of-nth-pos-and-rb-in-system-level-non-marking-mode
+  (implies (and (not (mv-nth 0 (las-to-pas l-addrs r-w-x (loghead 2 (xr :seg-visible 1 x86)) x86)))
+                (member-p addr l-addrs)
+                (canonical-address-listp l-addrs)
+                (equal bytes (mv-nth 1 (rb l-addrs r-w-x x86)))
+                (not (mv-nth 0 (rm08 addr r-w-x x86)))
+                (not (programmer-level-mode x86))
+                (not (page-structure-marking-mode x86))
+                (x86p x86))
+           (equal (mv-nth 1 (rm08 addr r-w-x x86))
+                  (nth (pos addr l-addrs) bytes)))
+  :hints (("Goal" :in-theory (e/d (pos rm08 member-p)
+                                  (signed-byte-p
+                                   (:meta acl2::mv-nth-cons-meta))))))
+
+(local
+ (defthmd rb-in-terms-of-nth-and-pos-in-system-level-non-marking-mode-helper
+   (implies
+    (and (signed-byte-p 48 lin-addr)
+         (not (mv-nth 0 (rb (list lin-addr) :x x86)))
+         (not (xr :programmer-level-mode 0 x86))
+         (not (xr :page-structure-marking-mode 0 x86))
+         (x86p x86))
+    (equal (car (mv-nth 1 (rb (list lin-addr) :x x86)))
+           (combine-bytes (mv-nth 1 (rb (list lin-addr) :x x86)))))
+   :hints (("Goal" :in-theory (e/d* () ((:meta acl2::mv-nth-cons-meta)))))))
+
+(defun find-info-from-program-at-term (thm mfc state)
+  (declare (xargs :stobjs (state) :mode :program)
+           (ignorable thm state))
+  (b* ((call (acl2::find-call-lst 'program-at (acl2::mfc-clause mfc)))
+       ((when (not call))
+        ;; (cw "~%~p0: Program-At term not encountered.~%" thm)
+        nil)
+       (addresses (cadr call))
+       ((when (not (equal (car addresses)
+                          'create-canonical-address-list)))
+        ;; (cw "~%~p0: Program-At without Create-Canonical-Address-List encountered.~%" thm)
+        nil)
+       (n (cadr addresses))
+       (prog-addr (caddr addresses))
+       (bytes (caddr call)))
+    `((n . ,n)
+      (prog-addr . ,prog-addr)
+      (bytes . ,bytes))))
+
+(defthm rb-in-terms-of-nth-and-pos-in-system-level-non-marking-mode
+  (implies (and (bind-free
+                 (find-info-from-program-at-term
+                  'rb-in-terms-of-nth-and-pos-in-system-level-non-marking-mode
+                  mfc state)
+                 (n prog-addr bytes))
+                (program-at (create-canonical-address-list n prog-addr) bytes x86)
+                (member-p lin-addr (create-canonical-address-list n prog-addr))
+                (syntaxp (quotep n))
+                (not (mv-nth 0 (rb (list lin-addr) :x x86)))
+                (not (programmer-level-mode x86))
+                (not (page-structure-marking-mode x86))
+                (x86p x86))
+           (equal (car (mv-nth 1 (rb (list lin-addr) :x x86)))
+                  (nth (pos lin-addr (create-canonical-address-list n prog-addr)) bytes)))
+  :hints (("Goal"
+           :do-not-induct t
+           :in-theory (e/d (program-at
+                            rb-in-terms-of-nth-and-pos-in-system-level-non-marking-mode-helper)
+                           (acl2::mv-nth-cons-meta
+                            rm08-to-rb
+                            member-p-canonical-address-p-canonical-address-listp))
+           :use ((:instance rm08-to-rb
+                            (r-w-x :x))
+                 (:instance member-p-canonical-address-p-canonical-address-listp
+                            (e lin-addr))
+                 (:instance rm08-in-terms-of-nth-pos-and-rb-in-system-level-non-marking-mode
+                            (addr lin-addr)
+                            (r-w-x :x)
+                            (l-addrs (create-canonical-address-list n prog-addr)))))))
+
+;; ======================================================================
+
+#||
+
+(defthm rb-wb-disjoint
+  (implies (and (disjoint-p addresses (strip-cars addr-lst))
+                (programmer-level-mode x86))
+           (equal (mv-nth 1 (rb addresses r-w-x (mv-nth 1 (wb addr-lst x86))))
+                  (mv-nth 1 (rb addresses r-w-x x86))))
+  :hints (("Goal" :in-theory (e/d (disjoint-p) ()))))
+
+(defthmd rb-wb-equal
+  (implies (and (equal addresses (strip-cars (remove-duplicate-keys addr-lst)))
+                (programmer-level-mode x86)
+                (addr-byte-alistp addr-lst))
+           (equal (mv-nth 1 (rb addresses r-w-x (mv-nth 1 (wb addr-lst x86))))
+                  (assoc-list addresses (reverse addr-lst))))
+  :hints (("Goal" :in-theory (e/d (wm08 rm08) ()))))
+
+(defthm rb-wb-subset
+  (implies (and (subset-p addresses (strip-cars addr-lst))
+                (programmer-level-mode x86)
+                ;; [Shilpi]: Ugh, this hyp. below is so annoying. I
+                ;; could remove it if I proved something like
+                ;; subset-p-strip-cars-of-remove-duplicate-keys,
+                ;; commented out below.
+                (canonical-address-listp addresses)
+                (addr-byte-alistp addr-lst))
+           (equal (mv-nth 1 (rb addresses r-w-x (mv-nth 1 (wb addr-lst x86))))
+                  (assoc-list addresses (reverse addr-lst))))
+  :hints (("Goal" :induct (assoc-list addresses (reverse addr-lst)))))
+
+(defthmd rb-rb-subset
+  ;; [Shilpi]: This theorem can be generalized so that the conclusion mentions
+  ;; addr1, where addr1 <= addr.  Also, this is an expensive rule. Keep it
+  ;; disabled generally.
+  (implies (and (equal (mv-nth 1 (rb (create-canonical-address-list i addr) r-w-x x86))
+                       bytes)
+                (canonical-address-p (+ -1 i addr))
+                (canonical-address-p addr)
+                (xr :programmer-level-mode 0 x86)
+                (posp i)
+                (< j i))
+           (equal (mv-nth 1 (rb (create-canonical-address-list j addr) r-w-x x86))
+                  (take j bytes)))
+  :hints (("Goal" :in-theory (e/d* (rb canonical-address-p signed-byte-p) ()))))
+
+(defthm rb-rb-split-reads
+  (implies (and (canonical-address-p addr)
+                (xr :programmer-level-mode 0 x86)
+                (natp j)
+                (natp k))
+           (equal (mv-nth 1 (rb (create-canonical-address-list (+ k j) addr) r-w-x x86))
+                  (append (mv-nth 1 (rb (create-canonical-address-list k addr) r-w-x x86))
+                          (mv-nth 1 (rb (create-canonical-address-list j (+ k addr)) r-w-x x86)))))
+  :hints (("Goal" :in-theory (e/d* (rb canonical-address-p signed-byte-p)
+                                   ((:meta acl2::mv-nth-cons-meta))))))
+
+(defthm program-at-wb-disjoint
+  (implies (and (programmer-level-mode x86)
+                (canonical-address-listp addresses)
+                (disjoint-p addresses (strip-cars addr-lst)))
+           (equal (program-at addresses r-w-x (mv-nth 1 (wb addr-lst x86)))
+                  (program-at addresses r-w-x x86)))
+  :hints (("Goal" :in-theory (e/d (program-at) (rb)))))
+
+(defthm program-at-pop-x86-oracle
+  (implies (programmer-level-mode x86)
+           (equal (program-at addresses r-w-x (mv-nth 1 (pop-x86-oracle x86)))
+                  (program-at addresses r-w-x x86)))
+  :hints (("Goal" :in-theory (e/d (program-at pop-x86-oracle pop-x86-oracle-logic)
+                                  (rb)))))
+
+(defthm program-at-write-user-rflags
+  (implies (programmer-level-mode x86)
+           (equal (program-at addresses r-w-x (write-user-rflags flags mask x86))
+                  (program-at addresses r-w-x x86)))
+  :hints (("Goal" :in-theory (e/d (write-user-rflags)
+                                  (force (force))))))
+
+
+(defthm wb-and-wb-combine-wbs
+  (implies (and (addr-byte-alistp addr-list1)
+                (addr-byte-alistp addr-list2)
+                (programmer-level-mode x86))
+           (equal (mv-nth 1 (wb addr-list2 (mv-nth 1 (wb addr-list1 x86))))
+                  (mv-nth 1 (wb (append addr-list1 addr-list2) x86))))
+  :hints (("Goal" :do-not '(generalize)
+           :in-theory (e/d (wb-and-wm08) (append acl2::mv-nth-cons-meta)))))
+
+(defthmd wb-remove-duplicate-writes
+  (implies (and (syntaxp
+                 (not
+                  (and (consp addr-list)
+                       (eq (car addr-list) 'remove-duplicate-keys))))
+                (addr-byte-alistp addr-list)
+                (programmer-level-mode x86))
+           (equal (wb addr-list x86)
+                  (wb (remove-duplicate-keys addr-list) x86)))
+  :hints (("Goal" :do-not '(generalize)
+           :in-theory (e/d (wm08)
+                           (acl2::mv-nth-cons-meta))
+           :induct (wb-duplicate-writes-induct addr-list x86))))
+
+(defthm rb-in-terms-of-nth-and-pos
+  (implies (and (bind-free (find-info-from-program-at-term
+                            'rb-in-terms-of-nth-and-pos
+                            mfc state)
+                           (n prog-addr bytes))
+                (program-at (create-canonical-address-list n prog-addr) bytes x86)
+                (member-p addr (create-canonical-address-list n prog-addr))
+                (syntaxp (quotep n))
+                (programmer-level-mode x86))
+           (equal (car (mv-nth 1 (rb (list addr) :x x86)))
+                  (nth (pos addr (create-canonical-address-list n prog-addr)) bytes)))
+  :hints (("Goal" :in-theory (e/d (program-at)
+                                  (acl2::mv-nth-cons-meta
+                                   rm08-in-terms-of-rb
+                                   member-p-canonical-address-p-canonical-address-listp
+                                   rb))
+           :use ((:instance rm08-in-terms-of-rb
+                            (r-w-x :x))
+                 (:instance member-p-canonical-address-p-canonical-address-listp
+                            (e addr))
+                 (:instance rm08-in-terms-of-nth-pos-and-rb
+                            (r-w-x :x)
+                            (addresses (create-canonical-address-list n prog-addr)))))))
+
+(defthm rb-in-terms-of-rb-subset-p
+  (implies
+   (and (bind-free (find-info-from-program-at-term
+                    'rb-in-terms-of-rb-subset-p
+                    mfc state)
+                   (n prog-addr bytes))
+        (program-at (create-canonical-address-list n prog-addr) bytes x86)
+        (subset-p addresses (create-canonical-address-list n prog-addr))
+        (consp addresses)
+        (syntaxp (quotep n))
+        (programmer-level-mode x86))
+   (equal (mv-nth 1 (rb addresses :x x86))
+          (append (list (nth (pos
+                              (car addresses)
+                              (create-canonical-address-list n prog-addr))
+                             bytes))
+                  (mv-nth 1 (rb (cdr addresses) :x x86)))))
+  :hints (("Goal"
+           :do-not-induct t
+           :in-theory (e/d (subset-p)
+                           (canonical-address-p
+                            acl2::mv-nth-cons-meta
+                            rb-in-terms-of-nth-and-pos))
+           :use ((:instance rb-unwinding-thm
+                            (r-w-x :x))
+                 (:instance rb-in-terms-of-nth-and-pos
+                            (addr (car addresses)))))))
+
+(defthm combine-bytes-rb-in-terms-of-rb-subset-p
+  (implies
+   (and (bind-free (find-info-from-program-at-term
+                    'combine-bytes-rb-in-terms-of-rb-subset-p
+                    mfc state)
+                   (n prog-addr bytes))
+        (program-at (create-canonical-address-list n prog-addr) bytes x86)
+        (subset-p addresses (create-canonical-address-list n prog-addr))
+        (consp addresses)
+        (syntaxp (quotep n))
+        (programmer-level-mode x86))
+   (equal
+    (combine-bytes (mv-nth 1 (rb addresses :x x86)))
+    (combine-bytes
+     (append (list (nth (pos (car addresses)
+                             (create-canonical-address-list n prog-addr))
+                        bytes))
+             (mv-nth 1 (rb (cdr addresses) :x x86))))))
+  :hints (("Goal" :in-theory (union-theories
+                              '()
+                              (theory 'minimal-theory))
+           :use ((:instance rb-in-terms-of-rb-subset-p)))))
+
+(globally-disable '(rb wb canonical-address-p program-at
+                       unsigned-byte-p signed-byte-p))
+
+||#
